done except for upgrade_gh, which is plausible but requires splicing

dev2015/dot-smallstep3a2.v
@@ -695,6 +695,11 @@ Lemma has_type_extend: forall GH G1 t T v n1,
   has_type GH (v::G1) t T n1.
 Proof. intros. eapply all_extend. eauto. eauto. Qed. 
 
+Lemma dms_has_type_extend: forall GH G1 t T v n1,
+  dms_has_type GH G1 t T n1 ->
+  dms_has_type GH (v::G1) t T n1.
+Proof. intros. eapply all_extend. eauto. eauto. Qed. 
+
 Lemma has_type_extend_mult: forall GH G1 t T G' n1,
   has_type GH G1 t T n1 ->
   has_type GH (G'++G1) t T n1.
@@ -718,11 +723,25 @@ Lemma has_type_closed: forall GH G1 t T n1,
   closed (length GH) (length G1) 0 T.
 Proof. intros. eapply all_closed with (t:=t). eauto. eauto. Qed.
 
+Lemma dms_has_type_closed: forall GH G1 t T n1,
+  dms_has_type GH G1 t T n1 ->
+  closed (length GH) (length G1) 0 T.
+Proof. intros. eapply all_closed with (ds:=t). eauto. eauto. Qed.
+
 Lemma has_type_closed_z: forall GH G1 z T n1,
   has_type GH G1 (tvar false z) T n1 ->
   z < length GH.
 Proof.
   intros. remember (tvar false z) as t. generalize dependent z.
+  induction H; intros; inversion Heqt; subst; eauto using index_max.
+Qed.
+
+
+Lemma has_type_closed1: forall GH G1 x T n1,
+  has_type GH G1 (tvar true x) T n1 ->
+  x < length G1.
+Proof.
+  intros. remember (tvar true x) as t. generalize dependent x.
   induction H; intros; inversion Heqt; subst; eauto using index_max.
 Qed.
 
@@ -1761,11 +1780,14 @@ Fixpoint subst_tm (u:nat) (T : tm) {struct T} : tm :=
   match T with
     | tvar true i         => tvar true i
     | tvar false i        => if beq_nat i 0 then (tvar true u) else tvar false (i-1)
-    | tobj (dty T)        => tobj (dty (subst (TVar true u) T))
-    | tobj (dfun T1 T2 t) => tobj (dfun (subst (TVar true u) T1) (subst (TVar true u) T2) (subst_tm u t))
+    | tobj ds             => tobj (subst_dm u ds)
     | tapp t1 t2          => tapp (subst_tm u t1) (subst_tm u t2)
+  end
+with subst_dm (u:nat) (d: dm) {struct d} : dm :=
+  match d with
+    | dty T        => dty (subst (TVar true u) T)
+    | dfun T1 T2 t => dfun (subst (TVar true u) T1) (subst (TVar true u) T2) (subst_tm u t)
   end.
-
 
 Inductive step : venv -> tm -> venv -> tm -> Prop :=
 | ST_Obj : forall G1 D,
@@ -1832,39 +1854,53 @@ Proof.
   eexists. eassumption.
 Qed.
 
-Lemma hastp_subst: forall m G1 GH TX T x t n1 n2,
-  has_type (GH++[TX]) G1 t T n2 ->
-  vtp m G1 x TX n1 ->
-  exists n3, has_type (map (substt x) GH) G1 (subst_tm x t) (substt x T) n3.
+Lemma hastp_upgrade_gh: forall G1 GH x T n1,
+  has_type [] G1 (tvar true x) T n1 ->
+  exists n, has_type GH G1 (tvar true x) T n.
 Proof.
-  intros. remember (GH++[TX]) as GH0. revert GH HeqGH0. induction H; intros.
-  - Case "varx". simpl. eexists. eapply T_Varx. erewrite subst_closed_id. eauto. eapply vtp_closed. eauto.
+  admit.
+Qed.
+
+Lemma hastp_subst_aux: forall ni, (forall G1 GH TX T x t n1 n2,
+  has_type (GH++[TX]) G1 t T n2 -> n2 < ni ->
+  has_type [] G1 (tvar true x) TX n1 ->
+  exists n3, has_type (map (substt x) GH) G1 (subst_tm x t) (substt x T) n3) /\
+  (forall G1 GH TX T x ds n1 n2,
+  dms_has_type (GH++[TX]) G1 ds T n2 -> n2 < ni ->
+  has_type [] G1 (tvar true x) TX n1 ->
+  exists n3, dms_has_type (map (substt x) GH) G1 (subst_dm x ds) (substt x T) n3).
+Proof.
+  intro ni. induction ni. split; intros; omega. destruct IHni as [IHniT IHniD].
+  split;
+  intros; remember (GH++[TX]) as GH0; revert GH HeqGH0; inversion H; intros.
+  - Case "varx". subst. simpl. eexists. eapply T_Varx. eauto. erewrite subst_closed_id. eauto. eapply dms_has_type_closed in H3. eauto.
   - Case "vary". subst. simpl.
     case_eq (beq_nat x0 0); intros E.
     + assert (x0 = 0). eapply beq_nat_true_iff; eauto. subst x0.
-      eexists. eapply T_Varx. eapply index_hit0 in H. subst. erewrite subst_closed_id. eauto. eapply vtp_closed. eauto. 
+      eapply index_hit0 in H2. subst.  erewrite subst_closed_id.
+      eapply hastp_upgrade_gh. eauto. eapply has_type_closed in H1. eauto.
     + assert (x0 <> 0). eapply beq_nat_false_iff; eauto.
-      eexists. eapply T_Vary. eapply index_subst1. eauto. eauto. rewrite map_length. eapply closed_subst0. rewrite app_length in H1. simpl in H1. eapply H1. eapply vtp_closed1. eauto.
+      eexists. eapply T_Vary. eapply index_subst1. eauto. eauto. rewrite map_length. eapply closed_subst0. rewrite app_length in H3. simpl in H3. eapply H3. eapply has_type_closed1. eauto.
   - Case "pack". subst. simpl.
-    simpl in IHhas_type. specialize (IHhas_type H0 GH0 eq_refl). ev.
+    edestruct IHniT as [? IH]. eauto. omega. eauto. 
     assert (substt x (TBind T1) = (TBind (substt x T1))) as A. {
       eauto.
     }
     rewrite A.
     destruct b.
-    + eexists. eapply T_VarPack. eapply H1.
+    + eexists. eapply T_VarPack. eapply IH.
       unfold substt. rewrite subst_open_commute1. reflexivity.
-      rewrite map_length. eapply closed_subst0. rewrite app_length in H2. simpl in H2.
-      apply H2. eapply vtp_closed1. eauto.
+      rewrite map_length. eapply closed_subst0. rewrite app_length in H4. simpl in H4.
+      apply H4. eapply has_type_closed1. eauto.
     + case_eq (beq_nat x0 0); intros E.
       * assert (x0 = 0). eapply beq_nat_true_iff; eauto. subst x0.
-        rewrite E in H1.
-        eexists. eapply T_VarPack. eapply H1. rewrite subst_open_commute0b. eauto.
-        rewrite map_length. eapply closed_subst. rewrite app_length in H2. simpl in H2.
-        eapply H2. econstructor. eapply vtp_closed1. eauto.
+        simpl in IH.
+        eexists. eapply T_VarPack. eapply IH. rewrite subst_open_commute0b. eauto.
+        rewrite map_length. eapply closed_subst. rewrite app_length in H4. simpl in H4.
+        eapply H4. econstructor. eapply has_type_closed1. eauto.
       * assert (x0 <> 0). eapply beq_nat_false_iff; eauto.
-        rewrite E in H1.
-        eexists. eapply T_VarPack. eapply H1.
+        simpl in IH. rewrite E in IH.
+        eexists. eapply T_VarPack. eapply IH.
         remember (x0 - 1) as z.
         assert (x0 = z + 1) as B. {
           intuition. destruct x0. specialize (H3 eq_refl). inversion H3.
@@ -1873,29 +1909,29 @@ Proof.
         }
         rewrite B. unfold substt.
         rewrite subst_open_commute_z. reflexivity.
-        rewrite map_length. eapply closed_subst. rewrite app_length in H2.
-        simpl in H2. eapply H2.
-        econstructor. eapply vtp_closed1. eauto.
+        rewrite map_length. eapply closed_subst. rewrite app_length in H4.
+        simpl in H4. eapply H4.
+        econstructor. eapply has_type_closed1. eauto.
   - Case "unpack". subst. simpl.
-    simpl in IHhas_type. specialize (IHhas_type H0 GH0 eq_refl). ev.
+    edestruct IHniT as [? IH]. eapply H2. omega. eauto.
     assert (substt x (TBind T1) = (TBind (substt x T1))) as A. {
       eauto.
     }
-    rewrite A in H1.
+    rewrite A in IH.
     destruct b.
-    + eexists. eapply T_VarUnpack. eapply H1.
+    + eexists. eapply T_VarUnpack. eapply IH.
       unfold substt. rewrite subst_open_commute1. reflexivity.
-      rewrite map_length. eapply closed_subst0. rewrite app_length in H2. simpl in H2.
-      apply H2. eapply vtp_closed1. eauto.
+      rewrite map_length. eapply closed_subst0. rewrite app_length in H4. simpl in H4.
+      apply H4. eapply has_type_closed1. eauto.
     + case_eq (beq_nat x0 0); intros E.
       * assert (x0 = 0). eapply beq_nat_true_iff; eauto. subst x0.
-        rewrite E in H1.
-        eexists. eapply T_VarUnpack. eapply H1. rewrite subst_open_commute0b. eauto.
-        rewrite map_length. eapply closed_subst. rewrite app_length in H2. simpl in H2.
-        eapply H2. econstructor. eapply vtp_closed1. eauto.
+        simpl in IH.
+        eexists. eapply T_VarUnpack. eapply IH. rewrite subst_open_commute0b. eauto.
+        rewrite map_length. eapply closed_subst. rewrite app_length in H4. simpl in H4.
+        eapply H4. econstructor. eapply has_type_closed1. eauto.
       * assert (x0 <> 0). eapply beq_nat_false_iff; eauto.
-        rewrite E in H1.
-        eexists. eapply T_VarUnpack. eapply H1.
+        simpl in IH. rewrite E in IH.
+        eexists. eapply T_VarUnpack. eapply IH.
         remember (x0 - 1) as z.
         assert (x0 = z + 1) as B. {
           intuition. destruct x0. specialize (H3 eq_refl). inversion H3.
@@ -1904,35 +1940,28 @@ Proof.
         }
         rewrite B. unfold substt.
         rewrite subst_open_commute_z. reflexivity.
-        rewrite map_length. eapply closed_subst. rewrite app_length in H2.
-        simpl in H2. eapply H2.
-        econstructor. eapply vtp_closed1. eauto.
-  - Case "mem". subst. simpl.
-    eexists. eapply T_Mem. eapply closed_subst0. rewrite app_length in H. rewrite map_length. eauto. eapply vtp_closed1. eauto.
-  - Case "abs". subst. simpl.
-    edestruct IHhas_type as [? HI]. eauto. instantiate (1:=T11::GH0). eauto.
-    simpl in HI. 
-    eexists. eapply T_Abs. eapply HI.
-    rewrite map_length. rewrite app_length. simpl.
-    rewrite subst_open. unfold substt. reflexivity.
-    eapply closed_subst0. rewrite map_length. rewrite app_length in H2. simpl in H2. eauto. eauto. eapply vtp_closed1. eauto.
-    eapply closed_subst0. rewrite map_length. rewrite app_length in H3. simpl in H3. eauto. eapply vtp_closed1. eauto.
-  - Case "app".
-    edestruct IHhas_type1. eauto. eauto.
-    edestruct IHhas_type2. eauto. eauto. 
+        rewrite map_length. eapply closed_subst. rewrite app_length in H4.
+        simpl in H4. eapply H4.
+        econstructor. eapply has_type_closed1. eauto.
+  - Case "obj". subst. simpl.
+    edestruct IHniD as [? IH]. eauto. omega. eauto.
+    eexists. eapply T_Obj. eauto. eapply dms_has_type_closed. eauto.
+  - Case "app". subst. simpl.
+    edestruct IHniT as [? IH1]. eapply H2. omega. eauto.
+    edestruct IHniT as [? IH2]. eapply H3. omega. eauto.
     eexists. eapply T_App. eauto. eauto. eapply closed_subst.
     subst. rewrite map_length. rewrite app_length in *. simpl in *. eauto.
-    subst. rewrite map_length. econstructor. eapply vtp_closed1. eauto.
-  - Case "appvar".
-    edestruct IHhas_type1. eauto. eauto.
-    edestruct IHhas_type2. eauto. eauto. simpl.
+    subst. rewrite map_length. econstructor. eapply has_type_closed1. eauto.
+  - Case "appvar". subst. simpl.
+    edestruct IHniT as [? IH1]. eapply H2. omega. eauto.
+    edestruct IHniT as [? IH2]. eapply H3. omega. eauto.
     destruct b2.
 
-    eexists. eapply T_AppVar. eauto. eauto. subst T2'.
+    eexists. eapply T_AppVar. eauto. eauto.
     rewrite subst_open_commute1. eauto.
     eapply closed_subst. subst. rewrite map_length. rewrite app_length in *. simpl in *.
     eapply closed_upgrade_gh. eassumption. omega.
-    subst. rewrite map_length. econstructor. eapply vtp_closed1. eauto.
+    subst. rewrite map_length. econstructor. eapply has_type_closed1. eauto.
 
     case_eq (beq_nat x2 0); intros E.
 
@@ -1942,21 +1971,40 @@ Proof.
     rewrite map_length. rewrite <- subst_open_commute0b.
     eapply closed_subst. eapply closed_upgrade_gh. eassumption.
     rewrite app_length. simpl. omega.
-    econstructor. eapply vtp_closed1. eauto.
+    econstructor. eapply has_type_closed1. eauto.
 
-    subst T2'. rewrite subst_open5.
+    rewrite subst_open5.
     simpl in *. rewrite E in *.
     eexists. eapply T_AppVar. eauto. eauto. eauto.
     rewrite <- subst_open5. eapply closed_subst.
     subst. rewrite map_length. rewrite app_length in *. simpl in *. eassumption.
-    subst. rewrite map_length. econstructor. eapply vtp_closed1. eauto.
+    subst. rewrite map_length. econstructor. eapply has_type_closed1. eauto.
     apply []. apply beq_nat_false. apply E. apply []. apply beq_nat_false. apply E.
   - Case "sub". subst.
-    edestruct stp2_subst_narrow. eapply H1. eapply H0.
-    edestruct IHhas_type. eauto. eauto.
+    edestruct hastp_inv as [? [? HV]]; eauto.
+    edestruct stp2_subst_narrow. eapply H3. eapply HV.
+    edestruct IHniT as [? IH]. eapply H2. omega. eauto.
     eexists. eapply T_Sub. eauto. eauto.
+  - Case "mem". subst. simpl.
+    eexists. eapply D_Mem. eapply closed_subst0. rewrite app_length in H2. rewrite map_length. eauto. eapply has_type_closed1. eauto.
+  - Case "abs". subst. simpl.
+    edestruct IHniT with (GH:=T11::GH1) as [? HI] . eauto. omega. eauto.
+    simpl in HI. 
+    eexists. eapply D_Abs. eapply HI.
+    rewrite map_length. rewrite app_length. simpl.
+    rewrite subst_open. unfold substt. reflexivity.
+    eapply closed_subst0. rewrite map_length. rewrite app_length in H4. simpl in H4. eauto. eauto. eapply has_type_closed1. eauto.
+    eapply closed_subst0. rewrite map_length. rewrite app_length in H5. simpl in H5. eauto. eapply has_type_closed1. eauto.
 Grab Existential Variables.
-  apply 0. apply 0.
+apply 0. apply 0.
+Qed.
+
+Lemma hastp_subst: forall G1 GH TX T x t n1 n2,
+  has_type (GH++[TX]) G1 t T n2 ->
+  has_type [] G1 (tvar true x) TX n1 ->
+  exists n3, has_type (map (substt x) GH) G1 (subst_tm x t) (substt x T) n3.
+Proof.
+  intros. eapply hastp_subst_aux with (t:=t). eauto. eauto. eauto.
 Qed.
 
 Theorem type_safety : forall G t T n1,
@@ -1977,22 +2025,10 @@ Proof.
   - Case "unpack". subst GH.
     eapply has_type_closed_b in H. destruct H. subst.
     left. eexists. reflexivity.
-  - Case "mem". right.
-    assert (stpd2 [] (vobj (dty T11)::G1) T11 T11).
-    eapply stpd2_refl. subst. eapply closed_extend. eauto. 
-    eu. repeat eexists. rewrite <-app_cons1. eapply ST_Obj. eapply T_Varx. eapply vtp_mem.
-    simpl. rewrite beq_nat_true_eq. eauto. eauto. eauto. 
-  - Case "abs". right.
-    inversion CL. subst.
-    assert (stpd2 [] (vobj (dfun T11 T12 t12)::G1) T11 T11).
-    eapply stpd2_refl. subst. eapply closed_extend. eauto.
-    assert (stpd2 [T11] (vobj (dfun T11 T12 t12)::G1) (open 0 (TVar false 0) T12) (open 0 (TVar false 0) T12)).
-    eapply stpd2_refl. subst. eapply closed_open. eapply closed_extend. simpl. eapply closed_upgrade_gh. simpl in *. eauto. omega. econstructor. simpl. omega.
-    eu. eu. repeat eexists. rewrite <-app_cons1. eapply ST_Obj. eapply T_Varx. eapply vtp_fun.
-    simpl. rewrite beq_nat_true_eq. eauto. subst.
-    eapply has_type_extend. eauto. eauto.
-    reflexivity. reflexivity.
-    eapply closed_extend. eauto. eapply closed_extend. eauto. eauto.
+  - Case "obj". subst. right.
+    repeat eexists. rewrite <- app_cons1. eapply ST_Obj. eapply T_Varx.
+    simpl. rewrite beq_nat_true_eq. eauto.
+    eapply dms_has_type_extend. eauto.
   - Case "app". subst.
     assert (closed (length ([]:tenv)) (length G1) 0 (TFun T1 T)) as TF. eapply has_type_closed. eauto. 
     assert ((exists x : id, t2 = tvar true x) \/
@@ -2087,9 +2123,6 @@ Proof.
     + SCase "step".
       ev. subst. 
       right. repeat eexists. eauto. eapply T_Sub. eauto. eapply stp2_extend_mult. eauto. 
-      
-Grab Existential Variables.
-apply 0. apply 0.
 Qed. 
 
 
